Tree and registers working again.  Roughly back to where I was a month ago.

Inserters/AndTree.dfy
@@ -6,15 +6,15 @@ module Inserters.AndTree{
   import opened Eval
   import opened ConservedSubcircuit
   import opened Utils
-  import opened Entity
+  import opened Scuf
   import opened MapFunction
   import opened ConnectionEval
   import opened Connection
-  import opened IslandBundle
   import opened Subcircuit
   import opened MapConnection
-  import opened CombineParallel
-  import opened CombineSeries
+  import opened ModifiersSeries
+  import opened Modifiers.Merge
+  import opened Modifiers.SwitchUF
 
   import opened And
   import opened Ident
@@ -53,303 +53,88 @@ module Inserters.AndTree{
     SO([AndTreeBehav(si.inputs)], [])
   }
 
-  ghost predicate MFReqs(n: nat, mf_a: MapFunction, mf_b: MapFunction, mf_and: MapFunction, mf_combined: MapFunction)
+  function AndTreeStep1UpdateFunction(n: nat): (uf: UpdateFunction)
+    requires n > 2
+    ensures uf.Valid()
   {
-    && n > 2
-    && var p := SubTreeSizes(n).0;
-    && AndTreeMFValid(p, mf_a)
-    && AndTreeMFValid(n-p, mf_b)
-    && AndMFValid(mf_and)
-    && AndTreeMFValid(n, mf_combined)
-    && mf_a.NPs() !! mf_b.NPs()
-    && mf_combined.inputs == mf_a.inputs + mf_b.inputs
-    && mf_and.inputs == mf_and.inputs == mf_a.outputs + mf_b.outputs
-    && mf_combined.outputs == mf_and.outputs
-  }
-
-  ghost predicate AndTreeMFValid(n: nat, mf: MapFunction)
-  {
-    && mf.Valid()
-    && (|mf.inputs| == n)
-    && (|mf.state| == 0)
-    && (|mf.outputs| == 1)
-    && (forall si :: SIValid(si, mf.inputs, mf.state) ==> (
-      && mf.sf.requires(si)
-      && (mf.sf(si) == AndTreeSF(n, si))))
-  }
-
-  function AndTreeMFImpl(n: nat, inputs: seq<NP>, output: NP): (mf: MapFunction)
-    requires |inputs| == n
-    requires Seq.HasNoDuplicates(inputs)
-    requires output !in inputs
-    ensures mf.Valid()
-    ensures AndTreeMFValid(n, mf)
-  {
-    reveal MapFunction.Valid();
-    reveal Seq.HasNoDuplicates();
-    reveal Seq.ToSet();
-    MapFunction(
-      inputs,
-      [output],
-      [],
-      (si: SI) requires SIValid(si, inputs, []) => AndTreeSF(n, si)
+    reveal UpdateFunction.Valid();
+    UpdateFunction(
+      n, 2, 0,
+      (si: SI) requires |si.inputs| == n && |si.state| == 0 =>
+        var p := SubTreeSizes(n).0;
+        var si1 := SI(si.inputs[..p], []);
+        var si2 := SI(si.inputs[p..], []);
+        SO(AndTreeSF(p, si1).outputs + AndTreeSF(n-p, si2).outputs, [])
     )
   }
 
-  function AndTreeMFFromEntities(c: Circuit, n: nat, e_left: Entity, e_right: Entity, e_and: Entity): (mf: MapFunction)
-    requires
-      && n > 2
-      && var p := SubTreeSizes(n).0;
-      && c.Valid()
-      && (e_left.sc !! e_right.sc)
-      && (e_left.sc !! e_and.sc)
-      && (e_right.sc !! e_and.sc)
-      && EntityValid(c, e_left)
-      && EntityValid(c, e_right)
-      && EntityValid(c, e_and)
-      && AndTreeMFValid(p, e_left.mf)
-      && AndTreeMFValid(n-p, e_right.mf)
-      //&& AndTreeMFValid(n, mf)
-      && AndMFValid(e_and.mf)
-      //&& mf.Valid()
-      //&& (mf.inputs == e_left.mf.inputs + e_right.mf.inputs)
-      //&& (mf.outputs == e_and.mf.outputs)
-    ensures
-      && reveal Seq.ToSet();
-      && (e_left.mf.NPs() !! e_right.mf.NPs())
-      && var mf_top := ParallelCombiner(e_left.mf, e_right.mf).mf();
-      && var series_combiner := SeriesCombiner(mf_top, e_and.mf);
-      && series_combiner.Valid()
-      && var mf_final := series_combiner.mf();
-      && mf_final.Valid()
-      && mf.Valid()
-      && AndTreeMFValid(n, mf)
-      && MapFunctionsEquiv(mf_final, mf)
+  function AndTreeUpdateFunction(n: nat): (uf: UpdateFunction)
+    ensures uf.Valid()
   {
-    assert e_left.sc !! e_right.sc;
-    assert e_left.sc !! e_and.sc;
-    assert e_right.sc !! e_and.sc;
-    assert EntityValid(c, e_left) && EntityValid(c, e_right) && EntityValid(c, e_and) by {
-      reveal IslandBundleValid();
-    }
-    FAllInSc(c, e_left);
-    FAllInSc(c, e_right);
-    FAllInSc(c, e_and);
-    ScNoIntersectionNPsNoIntersection(e_left.sc, e_right.sc, e_left.mf.NPs(), e_right.mf.NPs());
-    ScNoIntersectionNPsNoIntersection(e_left.sc, e_and.sc, e_left.mf.NPs(), e_and.mf.NPs());
-    ScNoIntersectionNPsNoIntersection(e_right.sc, e_and.sc, e_right.mf.NPs(), e_and.mf.NPs());
-    assert e_and.mf.outputs[0] !in e_left.mf.inputs + e_right.mf.inputs by {
-      reveal Seq.ToSet();
-      assert Seq.ToSet(e_and.mf.outputs) <= e_and.mf.NPs();
-      assert Seq.ToSet(e_left.mf.inputs) <= e_left.mf.NPs();
-      assert Seq.ToSet(e_right.mf.inputs) <= e_right.mf.NPs();
-      assert e_and.mf.outputs[0] !in Seq.ToSet(e_left.mf.inputs) + Seq.ToSet(e_right.mf.inputs);
-      assert e_and.mf.outputs[0] !in Seq.ToSet(e_left.mf.inputs + e_right.mf.inputs);
-      assert e_and.mf.outputs[0] !in e_left.mf.inputs + e_right.mf.inputs;
-    }
-    assert Seq.HasNoDuplicates(e_left.mf.inputs + e_right.mf.inputs) by {
-      reveal MapFunction.Valid();
-      NoDuplicatesInConcat(e_left.mf.inputs, e_right.mf.inputs);
-    }
-    var mf := AndTreeMFImpl(n, e_left.mf.inputs + e_right.mf.inputs, e_and.mf.outputs[0]);
-    AndTreeMFCorrect(n, e_left.mf, e_right.mf, e_and.mf, mf);
-    mf
+    reveal UpdateFunction.Valid();
+    UpdateFunction(
+      n, 1, 0,
+      (si: SI) requires |si.inputs| == n && |si.state| == 0 => AndTreeSF(n, si)
+    )
   }
 
-  lemma AndTreeMFCorrect(n: nat, mf_left: MapFunction, mf_right: MapFunction, mf_and: MapFunction, mf: MapFunction)
-    // Show the equivalence of a map function that gets built by doing combine parallel and combine series
-    // and the simpler map function that we'd like to replace it with.
-    requires
-      && n > 2
-      && var p := SubTreeSizes(n).0;
-      && AndTreeMFValid(p, mf_left)
-      && AndTreeMFValid(n-p, mf_right)
-      && AndTreeMFValid(n, mf)
-      && AndMFValid(mf_and)
-      && mf_left.NPs() !! mf_right.NPs()
-      && mf_left.NPs() !! mf_and.NPs()
-      && mf_right.NPs() !! mf_and.NPs()
-      && mf.Valid()
-      && mf.inputs == mf_left.inputs + mf_right.inputs
-      && mf.outputs == mf_and.outputs
-    ensures
-      && reveal Seq.ToSet();
-      && var mf_top := ParallelCombiner(mf_left, mf_right).mf();
-      && var series_combiner := SeriesCombiner(mf_top, mf_and);
-      && series_combiner.Valid()
-      && var mf_final := series_combiner.mf();
-      && mf_final.Valid()
-      && MapFunctionsEquiv(mf_final, mf)
-  {
-    var p := SubTreeSizes(n).0;
-    reveal Seq.ToSet();
-    var mf_top := ParallelCombiner(mf_left, mf_right).mf();
-    var series_combiner := SeriesCombiner(mf_top, mf_and);
-    assert series_combiner.Valid() by {
-      assert mf_top.Valid();
-      assert mf_and.Valid();
-      assert mf_top.NPs() <= mf_left.NPs() + mf_right.NPs() by {
-        reveal  Seq.ToSet();
-      }
-      assert (mf_top.NPs() !! mf_and.NPs());
-      assert (Seq.ToSet(mf_top.state) !! Seq.ToSet(mf_and.state));
-      assert (|mf_top.outputs| == |mf_and.inputs|);
-    }
-    var mf_final := series_combiner.mf();
-    assert mf_final.inputs == mf.inputs;
-    assert mf_final.outputs == mf.outputs;
-    assert mf_final.state == mf.state;
-    forall fi: FI | FIValid(fi, mf.inputs, mf.state)
-      ensures mf_final.f(fi) == mf.f(fi)
-    {
-      var si := mf.fi2si(fi);
-      assert mf.sf(si) == AndTreeSF(n, si);
-      var si_left := SI(si.inputs[..p], []);
-      var si_right := SI(si.inputs[p..], []);
-      reveal MapFunction.Valid();
-      assert |si_left.inputs| == |mf_left.inputs|;
-      assert |si_left.state| == |mf_left.state|;
-      var so_left := mf_left.sf(si_left);
-      var so_right := mf_right.sf(si_right);
-      var so_top := mf_top.sf(si);
-      assert so_top == SO(so_left.outputs + so_right.outputs, []);
-      var si_and := SI(so_left.outputs + so_right.outputs, []);
-      assert SIValid(si_and, mf_and.inputs, mf_and.state);
-      var so_and := mf_and.sf(si_and);
-      var so := SO(so_and.outputs, []);
-
-      assert so == mf_final.sf(si);
-
-      assert mf_final.sf(si) == mf.sf(si);
-      assert mf_final.f(fi) == mf.f(fi);
-    }
-    reveal MapFunctionsEquiv();
-  }
-
-  opaque function InsertAndTreeHelper(c: Circuit, n: nat): (r: (Circuit, Entity, MapFunction))
-    requires c.Valid()
-    requires n > 2
-    ensures r.0.Valid()
-    ensures EntityValid(r.0, r.1)
-    ensures CircuitUnconnected(c, r.0)
-    ensures CircuitConserved(c, r.0)
-    ensures IsIsland(r.0, r.1.sc)
-    ensures r.0.NodeKind.Keys == c.NodeKind.Keys + r.1.sc
-    ensures c.NodeKind.Keys !! r.1.sc
-    ensures |r.2.inputs| == n
-    ensures |r.2.outputs| == 1
-    ensures r.2.Valid()
-    ensures MapFunctionsEquiv(r.1.mf, r.2)
-    ensures AndTreeMFValid(n, r.2)
-    decreases n, 0
-  {
-    reveal SimpleInsertion();
-
-    var p := SubTreeSizes(n).0;
-    var eb1 := IslandBundleFromCircuit(c);
-
-    // Insert the left part of the tree.
-    var (c1, e_left) := InsertAndTreeImpl(c, p);
-    var (eb2, ref_left) := AddEntity(eb1, c1, e_left);
-
-    // Insert the right part of the tree.
-    var (c2, e_right) := InsertAndTreeImpl(c1, n-p);
-    var (eb3, ref_right) := AddEntity(eb2, c2, e_right);
-
-    // Insert an 'and' connecting them.
-    var (c3, e_and) := InsertAnd(c2);
-    var (eb4, ref_and) := AddEntity(eb3, c3, e_and);
-
-    // Join the left and rights parts in parallel
-    assert CombineParallelEntitiesRequirements(eb4.c, e_left, e_right) by {
-      reveal IslandBundleValid();
-    }
-    var (eb5, ref_top) := IBCombineParallelEntities(eb4, ref_left, ref_right);
-    var e_top := eb5.es[ref_top].value;
-
-    // Join the and on
-
-    assert CombineSeriesEntitiesRequirements(eb5.c, e_top, e_and) by {
-      reveal IslandBundleValid();
-      assert EntityValid(eb5.c, e_top);
-      assert e_and == eb5.es[ref_and].value;
-      assert EntityValid(eb5.c, e_and);
-    }
-    var (eb6, ref_final) := IBCombineSeriesEntities(eb5, ref_top, ref_and);
-    var e_final := eb6.es[ref_final].value;
-
-    var mf := AndTreeMFFromEntities(eb4.c, n, e_left, e_right, e_and);
-
-    assert CircuitUnconnected(c, eb6.c) by {
-      reveal IslandBundleValid();
-    }
-    assert CircuitConserved(c, eb6.c) by {
-      reveal IslandBundleValid();
-    }
-
-    assert eb6.c.NodeKind.Keys == c.NodeKind.Keys + e_final.sc by {
-      calc {
-        c1.NodeKind.Keys == c.NodeKind.Keys + e_left.sc;
-        c2.NodeKind.Keys == c1.NodeKind.Keys + e_right.sc;
-        c2.NodeKind.Keys == c.NodeKind.Keys + e_left.sc + e_right.sc;
-        c3.NodeKind.Keys == c2.NodeKind.Keys + e_and.sc;
-        c3.NodeKind.Keys == c.NodeKind.Keys + e_and.sc + e_left.sc + e_right.sc;
-        eb5.c.NodeKind.Keys == c.NodeKind.Keys + e_and.sc + e_left.sc + e_right.sc;
-        {assert e_top.sc == e_left.sc + e_right.sc;}
-        eb5.c.NodeKind.Keys == c.NodeKind.Keys + e_and.sc + e_top.sc;
-        eb6.c.NodeKind.Keys == c.NodeKind.Keys + e_and.sc + e_top.sc;
-        {assert e_final.sc == e_top.sc + e_and.sc;}
-        eb6.c.NodeKind.Keys == c.NodeKind.Keys + e_final.sc;
-      }
-    }
-
-    assert eb6.c.Valid() by {
-      reveal IslandBundleValid();
-    }
-    assert EntityValid(eb6.c, e_final) && IsIsland(eb6.c, e_final.sc) by {
-      reveal IslandBundleValid();
-    }
-    assert |e_final.mf.inputs| == n && |e_final.mf.outputs| == 1 by {
-      assert |e_left.mf.inputs| == p;
-      assert |e_right.mf.inputs| == n - p;
-      assert |e_top.mf.inputs| == n;
-    }
-
-    (eb6.c, e_final, mf)
-  }
-
-  opaque function InsertAndTreeImpl(c: Circuit, n: nat): (r: (Circuit, Entity))
-    requires c.Valid()
-    ensures r.0.Valid()
-    ensures EntityValid(r.0, r.1)
-    ensures CircuitUnconnected(c, r.0)
-    ensures CircuitConserved(c, r.0)
-    ensures IsIsland(r.0, r.1.sc)
-    ensures r.0.NodeKind.Keys == c.NodeKind.Keys + r.1.sc
-    ensures c.NodeKind.Keys !! r.1.sc
-    ensures AndTreeMFValid(n, r.1.mf)
+  lemma LemmaAndTreeUpdateFunction(n: nat)
+    ensures UpdateFunctionsEquiv(AndTreeInserterImpl(n).uf, AndTreeUpdateFunction(n))
     decreases n, 1
   {
-    if n == 0 then
-      InsertConst(c, true)
-    else if n == 1 then
-      InsertIdent(c)
-    else if n == 2 then
-      InsertAnd(c)
-    else
+    reveal UpdateFunctionsEquiv();
+    var uf1 := AndTreeInserterImpl(n).uf;
+    var uf2 := AndTreeUpdateFunction(n);
+    if n == 0 {
+      assert UpdateFunctionsEquiv(uf1, uf2);
+    } else if n == 1 {
+      assert UpdateFunctionsEquiv(uf1, uf2);
+    } else if n == 2 {
+      assert UpdateFunctionsEquiv(uf1, uf2);
+    } else {
+      assert n > 2;
       var p := SubTreeSizes(n).0;
-
-      var (new_c, e, mf) := InsertAndTreeHelper(c, n);
-
-      // Swap out the map function for a simpler one.
-      var new_e := EntitySwapMF(new_c, e, mf);
-      assert new_e.mf == mf;
-
-      reveal IslandBundleValid();
-      assert CircuitUnconnected(c, new_c);
-      assert CircuitConserved(c, new_c);
-
-      (new_c, new_e)
+      var z_left := AndTreeInserter(p);
+      var z_right := AndTreeInserter(n - p);
+      var z_left_and_right := MergeModifier(z_left, z_right);
+      assert UpdateFunctionsEquiv(AndTreeStep1UpdateFunction(n), z_left_and_right.uf) by {
+        reveal MergeUpdateFunctions();
+      }
+      var z_and := AndInserter();
+      var z := SeriesModifier(z_left_and_right, z_and);
+      assert UpdateFunctionsEquiv(uf1, uf2);
+    }
   }
 
+  function AndTreeInserterImpl(n: nat): (z: ScufInserter)
+    ensures z.Valid()
+    decreases n, 0
+  {
+    if n == 0 then
+      ConstInserter(true)
+    else if n == 1 then
+      IdentInserter()
+    else if n == 2 then
+      AndInserter()
+    else
+      var p := SubTreeSizes(n).0;
+      var z_left := AndTreeInserter(p);
+      var z_right := AndTreeInserter(n - p);
+      var z_left_and_right := MergeModifier(z_left, z_right);
+      var z_and := AndInserter();
+      var z := SeriesModifier(z_left_and_right, z_and);
+      z
+  }
+
+  function AndTreeInserter(n: nat): (z: ScufInserter)
+    ensures z.Valid()
+    decreases n, 2
+  {
+    var uf := AndTreeUpdateFunction(n);
+    var z_almost := AndTreeInserterImpl(n);
+    LemmaAndTreeUpdateFunction(n);
+    reveal UpdateFunctionsEquiv();
+    var z := SwitchUFModifier(z_almost, uf);
+    z
+  }
 }
