Modifiers/AppendReg.dfy
@@ -1,90 +1,66 @@
-module AppendReg {
+module ModifiersAppendReg {
     
   import opened Circ
-  import opened Entity
+  import opened Scuf
   import opened Subcircuit
   import opened ConservedSubcircuit
-  import opened IslandBundle
-  import opened Inserters.Reg
-  import opened CombineSeries
+  import opened InsertersReg
   import opened MapFunction
+  import opened ModifiersSeries
+  import opened Modifiers.SwitchUF
 
-  function AppendRegSF(rf_base: RFunction, si: SI): (so: SO)
+  function AppendRegSF(rf_base: UpdateFunction, si: SI): (so: SO)
     requires rf_base.Valid()
     requires |si.inputs| == rf_base.input_width && |si.state| == rf_base.state_width + rf_base.output_width
   {
     var si_base := SI(si.inputs, si.state[..rf_base.state_width]);
-    reveal RFunction.Valid();
+    reveal UpdateFunction.Valid();
     var so_base := rf_base.sf(si_base);
     var old_reg_state := si.state[|si_base.state|..];
     var so := SO(old_reg_state, so_base.state + so_base.outputs);
     so
   }
 
-  function AppendRegRF(rf_base: RFunction): (rf: RFunction)
-    requires rf_base.Valid()
-    ensures rf.Valid()
+  function AppendRegUpdateFunction(uf: UpdateFunction): (new_uf: UpdateFunction)
+    requires uf.Valid()
+    ensures new_uf.Valid()
   {
-    reveal RFunction.Valid();
-    RFunction(
-      rf_base.input_width,
-      rf_base.output_width,
-      rf_base.state_width + rf_base.output_width,
-      (si: SI) requires |si.inputs| == rf_base.input_width && |si.state| == rf_base.state_width + rf_base.output_width =>
-        AppendRegSF(rf_base, si)
+    reveal UpdateFunction.Valid();
+    UpdateFunction(
+      uf.input_width,
+      uf.output_width,
+      uf.state_width + uf.output_width,
+      (si: SI) requires |si.inputs| == uf.input_width && |si.state| == uf.state_width + uf.output_width =>
+        AppendRegSF(uf, si)
     )
   }
 
-  lemma RFEquiv(rf_base: RFunction)
-    requires rf_base.Valid()
+  lemma UFEquiv(uf: UpdateFunction)
+    requires uf.Valid()
     ensures
-      var reg_width := rf_base.output_width;
-      var rf_reg := RegRF(reg_width);
-      var rf_combined := CombineSeriesRF(rf_base, rf_reg);
-      var rf_appendreg := AppendRegRF(rf_base);
-      RFunctionEquiv(rf_appendreg, rf_combined)
+      var reg_width := uf.output_width;
+      var uf_reg := RegUpdateFunction(reg_width);
+      var uf_combined := SeriesUpdateFunction(uf, uf_reg);
+      var uf_appendreg := AppendRegUpdateFunction(uf);
+      UpdateFunctionsEquiv(uf_appendreg, uf_combined)
   {
-    reveal RFunction.Valid();
-    reveal RFunctionEquiv();
+    reveal UpdateFunction.Valid();
+    reveal UpdateFunctionsEquiv();
   }
 
-  function AppendReg(c: Circuit, ei: EntityInserter): (r: (Circuit, Entity))
-    requires c.Valid()
-    requires ei.Valid()
-    ensures SimpleInsertion(c, r.0, r.1)
-    ensures
-      reveal EntityInserter.Valid();
-      AppendRegRF(ei.rf).MFConsistent(r.1.mf)
+  function AppendRegModifier(z: ScufInserter): (new_z: ScufInserter)
+    requires z.Valid()
+    ensures new_z.Valid()
   {
-    var reg_width := ei.rf.output_width;
-    var ei_reg := RegInserter(reg_width);
-    var (c_a, e_a) := InsertTwoInSeries(c, ei, ei_reg);
-    assert ei.rf.Valid() by {
-      reveal EntityInserter.Valid();
+    reveal ScufInserter.Valid();
+    var z_reg := RegInserter(z.uf.output_width);
+    var z_series := SeriesModifier(z, z_reg);
+    var new_uf := AppendRegUpdateFunction(z.uf);
+    assert UpdateFunctionsEquiv(new_uf, z_series.uf) by {
+      UFEquiv(z.uf);
     }
-    var new_rf := AppendRegRF(ei.rf);
-    RFEquiv(ei.rf);
-    var rf_combined := CombineSeriesRF(ei.rf, ei_reg.rf);
-    assert c_a.Valid() && EntityValid(c_a, e_a) && e_a.mf.Valid() by {
-      reveal SimpleInsertion();
-    }
-    MFConsistentEquiv(rf_combined, new_rf, e_a.mf);
-    var e_b := EntitySwapRF(c_a, e_a, new_rf);
-    assert SimpleInsertion(c, c_a, e_b) by {
-      reveal SimpleInsertion();
-    }
-    (c_a, e_b)
-  }
-
-  function AppendRegInserter(ei_base: EntityInserter): (ei: EntityInserter)
-    requires ei_base.Valid()
-    ensures ei.Valid()
-  {
-    reveal EntityInserter.Valid();
-    EntityInserter(
-      AppendRegRF(ei_base.rf),
-      (c: Circuit) requires c.Valid() => AppendReg(c, ei_base)
-    )
+    var new_z := SwitchUFModifier(z_series, new_uf);
+    new_z
   }
 
 }
