Inserters/Null.dfy
@@ -1,0 +1,53 @@
+module Inserters.Null {
+
+  import opened Circ
+  import opened Scuf
+  import opened MapFunction
+  import opened ConservedSubcircuit
+  import opened Subcircuit
+
+  //function NullUpdateFunction(): (r: UpdateFunction)
+  //  ensures r.Valid()
+  //{
+  //  reveal UpdateFunction.Valid();
+  //  UpdateFunction(0, 0, 0, (si: SI) requires |si.inputs| == 0 && |si.state| == 0 => SO([], []))
+  //}
+
+  function NullScufMap(): (mp: ScufMap)
+    ensures mp.Valid()
+  {
+    reveal Seq.HasNoDuplicates();
+    reveal Seq.ToSet();
+    ScufMap([], [], [])
+  }
+
+  function NullScuf(): (s: Scuf)
+  {
+    Scuf({}, NullScufMap(), NullUpdateFunction())
+  }
+
+  function NullInserter(): (z: ScufInserter)
+    ensures z.Valid()
+  {
+    reveal ScufInserter.Valid();
+    reveal SimpleInsertion();
+    var z := ScufInserter(NullUpdateFunction(), (c: Circuit) => (c, NullScuf()));
+    assert z.Valid() by {
+      assert z.uf.Valid();
+      forall c: Circuit | c.Valid()
+        ensures z.SpecificValid(c)
+      {
+        reveal IsIsland();
+        reveal CircuitUnconnected();
+        reveal CircuitConserved();
+        reveal Circuit.Valid();
+        reveal ScValid();
+        reveal Scuf.SomewhatValid();
+        reveal Scuf.EvaluatesCorrectly();
+        reveal NPsInSc();
+        reveal Seq.ToSet();
+      }
+    }
+    z
+  }
+}
