Modifiers/ManyParallel.dfy
@@ -1,0 +1,191 @@
+module Modifiers_ManyParallel {
+
+  import opened Std.Wrappers
+  import Std.Collections.Seq
+
+  import opened MapFunction
+  import opened MapConnection
+  import opened Utils
+  import opened Circ
+  import opened Scuf
+  import opened Subcircuit
+  import opened Connection
+  import opened ConservedSubcircuit
+  import opened Inserters.Null
+  import opened Modifiers.Merge
+  import opened Modifiers.SwitchUF
+
+  lemma ManyParallelSFOne(uf: UpdateFunction, si: SI)
+    requires uf.Valid()
+    requires |si.inputs| == uf.input_width 
+    requires |si.state| == uf.state_width
+    ensures
+      reveal UpdateFunction.Valid();
+      ManyParallelSF(uf, 1, si) == uf.sf(si)
+  {
+    var nm1_si := SI(si.inputs[uf.input_width..], si.state[uf.state_width..]);
+    var n_si := SI(si.inputs[..uf.input_width], si.state[..uf.state_width]);
+    var nm1_so := ManyParallelSF(uf, 0, nm1_si);
+    assert |nm1_so.outputs| == 0;
+    assert |nm1_so.state| == 0;
+    reveal UpdateFunction.Valid();
+    var n_so := uf.sf(n_si);
+    var so := SO(n_so.outputs + nm1_so.outputs, n_so.state + nm1_so.state);
+    assert n_si == si;
+    assert uf.sf(n_si) == SO(n_so.outputs, n_so.state);
+    assert so == uf.sf(si);
+  }
+
+  function {:vcs_split_on_every_assert} ManyParallelSF(uf: UpdateFunction, n: nat, si: SI): (so: SO)
+    requires |si.inputs| == uf.input_width * n
+    requires |si.state| == uf.state_width * n
+    requires uf.Valid()
+    ensures |so.outputs| == uf.output_width * n
+    ensures |so.state| == uf.state_width * n
+    decreases n
+  {
+    if n == 0 then
+      SO([], [])
+    else
+      var nm1_si := SI(si.inputs[uf.input_width..], si.state[uf.state_width..]);
+      var n_si := SI(si.inputs[..uf.input_width], si.state[..uf.state_width]);
+      var nm1_so := ManyParallelSF(uf, n-1, nm1_si);
+      reveal UpdateFunction.Valid();
+      var n_so := uf.sf(n_si);
+      SO(n_so.outputs + nm1_so.outputs, n_so.state + nm1_so.state)
+  }
+
+  function UpdateFunctionByMerge(uf: UpdateFunction, n: nat): (new_uf: UpdateFunction)
+    requires uf.Valid()
+    ensures new_uf.Valid()
+  {
+    if n == 0 then
+      NullUpdateFunction()
+    else if n == 1 then
+      uf
+    else
+      var uf_other := UpdateFunctionByMerge(uf, n-1);
+      var new_uf := MergeUpdateFunctions(uf, uf_other);
+      new_uf
+  }
+
+  function ManyParallelUpdateFunction(uf: UpdateFunction, n: nat): (new_uf: UpdateFunction)
+    requires uf.Valid()
+    ensures new_uf.Valid()
+    ensures new_uf.input_width == n * uf.input_width
+    ensures new_uf.output_width == n * uf.output_width
+    ensures new_uf.state_width == n * uf.state_width
+  {
+    var new_uf := UpdateFunction(
+      n * uf.input_width,
+      n * uf.output_width,
+      n * uf.state_width,
+      (si: SI) requires |si.inputs| == n * uf.input_width && |si.state| == n * uf.state_width
+        => ManyParallelSF(uf, n, si)
+    );
+    assert new_uf.Valid() by {
+      forall si: SI | new_uf.SIVal(si) {
+        assert new_uf.sf.requires(si);
+        assert new_uf.SOVal(new_uf.sf(si));
+      }
+      reveal UpdateFunction.Valid();
+    }
+    new_uf
+  }
+
+  lemma ManyParallelUpdateFunctionCorrect(z: ScufInserter, n: nat)
+    requires z.Valid()
+    ensures
+      reveal ScufInserter.Valid();
+      var uf1 := ManyParallelUpdateFunction(z.uf, n);
+      var uf2 := ManyParallelInserterImpl(z, n).uf;
+      UpdateFunctionsEquiv(uf1, uf2)
+    decreases n, 1
+  {
+    reveal ScufInserter.Valid();
+    reveal UpdateFunction.Valid();
+    var uf1 := ManyParallelUpdateFunction(z.uf, n);
+    var uf2 := ManyParallelInserterImpl(z, n).uf;
+    assert uf1.input_width == uf2.input_width;
+    assert uf1.output_width == uf2.output_width;
+    assert uf1.state_width == uf2.state_width;
+    reveal UpdateFunctionsEquiv();
+    if n == 0 {
+      assert UpdateFunctionsEquiv(uf1, uf2);
+    } else if n == 1 {
+      assert uf2 == z.uf;
+      forall si: SI | |si.inputs| == uf1.input_width && |si.state| == uf1.state_width
+        ensures uf1.sf(si) == uf2.sf(si)
+      {
+        ManyParallelSFOne(z.uf, si);
+      }
+      assert UpdateFunctionsEquiv(uf1, uf2);
+    } else {
+      assert uf2 == MergeUpdateFunctions(z.uf, ManyParallelUpdateFunction(z.uf, n-1)) by {
+        var z_other := ManyParallelInserter(z, n-1);
+        var z_merged := MergeModifier(z, z_other);
+        assert z_merged.uf == uf2;
+      }
+      forall si: SI | |si.inputs| == uf1.input_width && |si.state| == uf1.state_width
+        ensures uf1.sf(si) == uf2.sf(si)
+      {
+        assert uf1.sf.requires(si);
+        assert uf2.sf.requires(si);
+        assert uf1.sf(si) == ManyParallelSF(z.uf, n, si);
+        var si_this := SI(si.inputs[..z.uf.input_width], si.state[..z.uf.state_width]);
+        var so_this := z.uf.sf(si_this);
+        var si_other := SI(si.inputs[z.uf.input_width..], si.state[z.uf.state_width..]);
+        var uf1_other := ManyParallelUpdateFunction(z.uf, n-1);
+        var uf2_other := ManyParallelInserterImpl(z, n-1).uf;
+        var so1_other := uf1_other.sf(si_other);
+        var so2_other := uf2_other.sf(si_other);
+        ManyParallelUpdateFunctionCorrect(z, n-1);
+        assert so1_other == so2_other;
+        var so1_combined := SO(so_this.outputs + so1_other.outputs, so_this.state + so1_other.state);
+        assert so1_combined == uf1.sf(si);
+        assert so1_combined == uf2.sf(si) by {
+          reveal MergeUpdateFunctions();
+          assert uf2 == MergeUpdateFunctions(z.uf, uf1_other);
+        }
+        assert uf1.sf(si) == uf2.sf(si);
+      }
+      assert UpdateFunctionsEquiv(uf1, uf2);
+    }
+    assert UpdateFunctionsEquiv(uf1, uf2);
+  }
+
+  function ManyParallelInserterImpl(z: ScufInserter, n: nat): (new_z: ScufInserter)
+    requires z.Valid()
+    ensures new_z.Valid()
+    ensures new_z.uf.input_width == z.uf.input_width * n
+    ensures new_z.uf.output_width == z.uf.output_width * n
+    ensures new_z.uf.state_width == z.uf.state_width * n
+    decreases n, 0
+  {
+    reveal ScufInserter.Valid();
+    var new_z := if n == 0 then
+      var z_null := NullInserter();
+      z_null
+    else if n == 1 then
+      z
+    else
+      var z_other := ManyParallelInserter(z, n-1);
+      var z_merged := MergeModifier(z, z_other);
+      z_merged;
+    new_z
+  }
+
+  function ManyParallelInserter(z: ScufInserter, n: nat): (new_z: ScufInserter)
+    requires z.Valid()
+    ensures new_z.Valid()
+    decreases n, 2
+  {
+    var z_almost := ManyParallelInserterImpl(z, n);
+    reveal ScufInserter.Valid();
+    var new_uf := ManyParallelUpdateFunction(z.uf, n);
+    reveal MergeUpdateFunctions();
+    ManyParallelUpdateFunctionCorrect(z, n);
+    var new_z := SwitchUFModifier(z_almost, new_uf);
+    new_z
+  }
+}
